comments

showcase.v
@@ -6,7 +6,8 @@ Local Open Scope string.
 Import ListNotations MCMonadNotation Nat.
 
 Inductive rose : Prop := Node (xs:list rose).
-Inductive roseA (A:Type) : Prop := LeafA (a:A) | NodeA (xs:list (roseA A)).
+Inductive list2 (A:Type) := nil2 | cons2 (a:A) (xs:list2 A).
+Inductive roseA (A:Type) : Type := LeafA (a:A) | NodeA (xs:list2 (roseA A)).
 
 From MetaCoq.Translations Require Import translation_utils.
 From MetaCoq.Translations Require Import param_original.
@@ -21,15 +22,71 @@ Print listᵗ.
 MetaCoq Run (TC <- Translate list_TC "rose" ;;
                 tmDefinition "rose_TC" TC ).
 Print roseᵗ.
-MetaCoq Run (TC <- Translate list_TC "roseA" ;;
+MetaCoq Run (TC <- Translate list_TC "list2" ;;
+                tmDefinition "list2_TC" TC ).
+MetaCoq Run (TC <- Translate list2_TC "roseA" ;;
                 tmDefinition "roseA_TC" TC ).
 Print roseAᵗ.
 
 MetaCoq Run (createIH false listᵗ).
+MetaCoq Run (createIH false list2ᵗ).
 Print listᵗ_nested_ind.
 Fail MetaCoq Run (createIH false roseᵗ).
 MetaCoq Run (createFunctorial false listᵗ).
 MetaCoq Run (createIH false roseᵗ).
 Print roseᵗ_nested_ind.
+MetaCoq Run (createFunctorial false list2ᵗ).
 MetaCoq Run (createIH false roseAᵗ).
 Print roseAᵗ_nested_ind.
+
+
+Lemma nat_natᵗ n: natᵗ n.
+    induction n;constructor;auto.
+Defined.
+
+Lemma list_listᵗ A P: (forall a, P a) -> forall x, listᵗ A P x.
+    induction x;constructor;auto.
+Defined.
+
+Lemma list2_list2ᵗ A P: (forall a, P a) -> forall x, list2ᵗ A P x.
+    induction x;constructor;auto.
+Defined.
+
+Lemma roseA_roseAᵗ A P: (forall a, P a) -> forall x, roseAᵗ A P x.
+Admitted.
+
+Goal roseA nat -> True.
+    intros r.
+    assert(roseAᵗ nat natᵗ r).
+    {
+        assert(forall n, natᵗ n).
+        {
+            induction n;constructor;auto.
+        }
+
+    }
+
+
+Goal roseA nat -> True.
+    intros r.
+    assert(roseAᵗ nat natᵗ r).
+    {
+        induction r.
+        - constructor. induction a;constructor;auto.
+        - constructor.
+          induction xs.
+          + constructor.
+          + constructor.
+    admit.
+    }
+    induction H using roseAᵗ_nested_ind.
+    - admit.
+    - admit.
+
+Goal rose -> nat.
+    intros r.
+    assert (roseᵗ r).
+    {
+        induction r.
+    }
+    induction r using roseᵗ_nested_ind.
