functorial.v
@@ -1,3 +1,53 @@
+(**
+Creates functorial lemmas that the parametricity translation
+behaves like a functor in respect to its parameters
+
+Application: When proving the induction lemma, 
+one encounters the problem that the parametricity translation argument
+listᵗ rose roseᵗ H is given stating that the property roseᵗ holds for all rose
+trees in the list. But we want the nested inductive hypothesis
+listᵗ rose P H that the property P under consideration in the induction
+holds for all trees in the list.
+Therefore, we need to translate the proofs of roseᵗ to P.
+This is possible for two reasons:
+* The inductive proof transforms roseᵗ instances into proofs of P
+    (we state that P holds for all roseᵗ)
+* Secondly, the parametricity translation of a container simply boundles
+    all proofs for the elements in it.
+  Therefore, all proofs can be replaced for another property, and thus,
+  the parametricity translation of a container behaves like a functor.
+
+Note: The substitution of P for roseᵗ makes it clear why
+    the induction does not carry the roseᵗ instances in the predicate
+    as such handling for nested types would no longer be possible.
+    Additionally, the generates lemma is less cluttered as it is ultimately
+    a lemma for rose not roseᵗ.
+
+example:
+listᵗ A Aᵗ x
+with A:Type, Aᵗ:A->Type, x:list A
+
+the functorial lemma has type:
+∀ A (Aᵗ:A->Type) (Aᵗ':A->Type) (F_A: ∀ (a:A), Aᵗ a -> Aᵗ' a)
+(x:list A),
+listᵗ A Aᵗ x -> listᵗ A Aᵗ' x
+
+Note:
+A->Type can be viewed as (Typeᵗ A)
+
+For each pair of parameter and translation another translation as destination
+is introduced together with a function stating the translation property for this paramter.
+This property will be recursively instantiated in the proofs.
+If the parameter has no arguments or does not result in a sort, a dummy value like True
+is introduced as each parametricity translated argument contains the same information.
+
+The indices contain no further information needed to be transferred between instances.
+They do not possess a functorial nature as they are dictated by inversion.
+Therefore, they are carried over.
+A special indice is the instance of the original type (list in the example above).
+But this instance does not need any special care.
+
+*)
 Require Import util.
 
 From MetaCoq.Template Require Import All.
@@ -41,6 +91,12 @@ Section Functorial.
         TemplateToPCUIC.trans [] <% True %>.
 
 
+    (*
+    given an argument Aᵗ generates the functorial property term
+    for ∀, copy the binder and remember to apply the arguments
+    for Sort, generate Aᵗ args -> Aᵗ' args 
+    Otherwise generate True
+     *)
         (* this is something like parametricity itself *)
     Fixpoint func x y args t :=
         match t with
@@ -53,11 +109,16 @@ Section Functorial.
         | _ => TrueQ
         end.
 
-    Variant augmentation {T:Type} := Norm (t:T) | Aug (t:T).
 
     Definition app_arg_list num args := map (fun x => x+num) args++mkNums num.
 
-    (* no context *)
+    (* no context but list of params *)
+    (* 
+    for params A, Aᵗ add Aᵗ' and F_A
+    takes list of param applications for the original and transformed term
+    returns the number of parameter groups, the list of argument applications
+    as number for the binder and lastly the list of new arguments (params & indices)
+     *)
     Fixpoint augment (params:context) (arg1 arg2:list nat):= 
         match params with
         | x::xᵗ::xr => 
@@ -77,33 +138,14 @@ Section Functorial.
             app_arg_list (#|params|+#|indices|) arg2),params++indices)
         end.
 
-    (* Fixpoint re_lift (xs:list(@augmentation (BasicAst.context_decl term))) : list (BasicAst.context_decl term) :=
-        match xs with
-        | [] => []
-        | Norm x::xs => x::re_lift xs
-        | Aug x::xs =>
-            x::mapi (fun i a =>
-                map_decl (lift 1 i) a
-            ) 
-            (re_lift xs)
-        end. *)
-
+        (* computes number of param groups and type of the functorial property *)
     Definition type_ := 
         let '((groups,arg1,arg2),aug_args) := augment (rev param_ctx) [] [] in
         let aug_args_ctx := rev (aug_args) in
         (groups,
-        (* let arg1' := app_arg_list #|indice_ctx| arg1 in
-        let arg2' := app_arg_list #|indice_ctx| arg2 in *)
         it_mkProd_or_LetIn 
             aug_args_ctx
-        (* it_mkProd_or_LetIn 
-        (
-            lift_context (2*groups) 0 indice_ctx ++
-            aug_param_ctx 
-        )  *)
         (tProd rAnon
-        (* TrueQ *)
-        (* (mkApps ind_term [tRel 4;tRel 3;tRel 0]) *)
         (mkApps ind_term (map tRel arg1))
         (lift0 1 (mkApps ind_term (map tRel arg2)))
         ))
@@ -117,7 +159,12 @@ Section Functorial.
     Definition functorial_type :=
     PCUICToTemplate.trans type.
 
-    Definition functorial :=
+    (*
+    Generation of the functorial property 
+    currently, the properties are only realized 
+    using obligations
+     *)
+    (* Definition functorial :=
     tCast 
     (PCUICToTemplate.trans
         placeholder
@@ -126,7 +173,7 @@ Section Functorial.
         ) *)
     )
     Cast
-    (PCUICToTemplate.trans type).
+    (PCUICToTemplate.trans type). *)
     
 End Functorial.
 
