util.v
@@ -1,10 +1,13 @@
+(**
+Provides commonly needed auxiliary definitions
+*)
 From MetaCoq.Template Require Import All.
 
 From MetaCoq Require Import All.
 Require Import String List.
-(* Local Open Scope string. *)
 Import ListNotations Nat.
 Import MCMonadNotation.
+Import IfNotations.
 
 From MetaCoq.PCUIC Require Import 
      PCUICAst PCUICAstUtils PCUICInduction
@@ -14,6 +17,7 @@ From MetaCoq.PCUIC Require Import
 From MetaCoq.PCUIC Require Import TemplateToPCUIC.
 From MetaCoq.PCUIC Require Import PCUICToTemplate.
 
+(* quick way to handle new naming with relevance *)
 Definition relevant_binder (n:name) :=
     {|
     binder_name := n;
@@ -21,6 +25,15 @@ Definition relevant_binder (n:name) :=
     |}.
 Definition rAnon := relevant_binder nAnon.
 Definition rName n := relevant_binder (nNamed n).
+
+Definition extendName prefix (n:name) suffix :=
+    match n with 
+    | nAnon => nAnon
+    | nNamed id => nNamed (prefix^id^suffix)
+    end.
+Definition extendAname prefix n suffix:= 
+    map_binder_annot (fun n => extendName prefix n suffix) n.
+
 (* generates a list (n-1), ..., 0 *)
 Fixpoint mkNums (n:nat) :=
     match n with 
@@ -28,10 +41,89 @@ Fixpoint mkNums (n:nat) :=
     | S m => [m] ++ mkNums m
     end.
 (* generates a list tRel (n-1), ..., tRel 0 *)
+(* useful to apply a bunch of arguments quantified with binders directly in front *)
 Fixpoint mkRels (n:nat) := map tRel (mkNums n).
 Fixpoint mkAstRels (n:nat) := map Ast.tRel (mkNums n).
 
+(* hole like underscores to be inferred
+  only work in limited cirumstances
+  a way that works is to compute the type
+  and use holes in the body which is casted to have the correct type
+  but then holes can not be used inside the type
+
+  some tricks are possible: for instance 
+  when creating lambdas (for instance with eta_expansion) that
+  are sure to be instanciated using beta reduction, one
+  can use dummy values in the lambdas and eagerly (with mkEagerApp)
+*)
 Definition hole := tEvar fresh_evar_id [].
-Variable (TODO: forall {T}, T).
+
+(* can be quoted as more powerful hole (coq does not need to fill it in)
+    only for testing/debugging purposes
+ *)
+(* Variable (TODO: forall {T}, T).
 Definition AstPlaceholder := Ast.mkApp <% @TODO %> (Ast.hole).
-Definition placeholder := TemplateToPCUIC.trans [] AstPlaceholder.
+Definition placeholder := TemplateToPCUIC.trans [] AstPlaceholder. *)
+
+
+
+(*
+n = destination
+k = local binder count
+
+works like subst: replaces binders behind n with an instance from s
+if s is large enough otherwise, reduce the binder to simulate instantiation
+*)
+Fixpoint local_subst_ (s:list term) (n:nat) (k:nat) (t:term) := 
+  match t with
+  | tRel m =>
+      (* difference: correct distance is dest (n)+local (k) *)
+	  if k+n <=? m
+      then
+        (* difference: only lift over local binders *)
+        if nth_error s (m - k-n) is Some b then lift0 k b else tRel (m - #|s|)
+      else tRel m
+  | tEvar ev args => tEvar ev (map (local_subst_ s n k) args)
+  | tProd na A B => tProd na (local_subst_ s n k A) (local_subst_ s n (S k) B)
+  | tLambda na T M => tLambda na (local_subst_ s n k T) (local_subst_ s n (S k) M)
+  | tLetIn na b ty b' =>
+      tLetIn na (local_subst_ s n k b) (local_subst_ s n k ty) (local_subst_ s n (S k) b')
+  | tApp u0 v => tApp (local_subst_ s n k u0) (local_subst_ s n k v)
+  | tCase ind p c brs =>
+      let p' := map_predicate_k id (local_subst_ s n) k p in
+      let brs' := map_branches_k (local_subst_ s n) id k brs in
+      tCase ind p' (local_subst_ s n k c) brs'
+  | tProj p c => tProj p (local_subst_ s n k c)
+  | tFix mfix idx =>
+      let k' := #|mfix| + k in
+      let mfix' := map (map_def (local_subst_ s n k) (local_subst_ s n k')) mfix in
+      tFix mfix' idx
+  | tCoFix mfix idx =>
+      let k' := #|mfix| + k in
+      let mfix' := map (map_def (local_subst_ s n k) (local_subst_ s n k')) mfix in
+      tCoFix mfix' idx
+  | _ => t
+  end.
+
+Definition local_subst s n := local_subst_ s n 0.
+
+
+
+(*
+performs beta reduction if directly applicable
+otherwise, introduce application
+*)
+(* TODO: there once was a function doing this already (was it mkApp in a previous version?) *)
+Definition mkEagerApp (a:term) (b:term) : term :=
+    match a with 
+    (* we completely ignore the type of the lambda as we might eliminate an error or at least do not introduce one *)
+    | tLambda na _ body =>
+        body {0:=b}
+    | _ => tApp a b 
+    end.
+
+Fixpoint mkEagerApps (t:term) (us:list term) : term :=
+    match us with
+    | [] => t
+    | u::ur => mkEagerApps (mkEagerApp t u) ur
+    end.
