ReadMe.md
@@ -1,0 +1,12 @@
+# Nested Induction V2
+
+A version of nested induction in MetaCoq which follows "Deriving proved equality tests in Coq-elpi: Stronger induction principles for containers in Coq" by Enrico Tassi.
+
+# TODO
+* automatic generation of proofs for functorial lemma
+* remove clutter
+* showcase how to use the lemmas (create indᵗ instance)
+* user friendly commands
+* use new parametricity
+* describe file in ReadMe
+* fully update induction.v comments to new version
